safechecker/theories/PCUICTypeChecker.v
@@ -1427,8 +1427,8 @@ Section Typecheck.
       | (primFloat; primFloatModel f) := ret _
       | (primString; primStringModel f) := ret _
       | (primArray; primArrayModel a) :=
-        check_eq_true (abstract_env_ext_wf_universeb X (Universe.of_level a.(array_level))) (Msg "primitive array level is not well-formed") ;;
-        check_type <- bdcheck infer Γ wfΓ a.(array_type) (tSort (sType (Universe.of_level a.(array_level)))) _ ;;
+        check_eq_true (abstract_env_ext_wf_universeb X (Universe.of_level a.(array_universe))) (Msg "primitive array level is not well-formed") ;;
+        check_type <- bdcheck infer Γ wfΓ a.(array_type) (tSort (sType (Universe.of_level a.(array_universe)))) _ ;;
         check_default <- bdcheck infer Γ wfΓ a.(array_default) a.(array_type) _ ;;
         check_values <- make_All (fun x => bdcheck infer Γ wfΓ x a.(array_type) _) a.(array_value) ;;
         ret _.
@@ -1453,7 +1453,7 @@ Section Typecheck.
         now move/@wf_universe_reflect: i.
       - specialize (check_type _ wfΣ) as [].
         specialize (check_default _ wfΣ) as [].
-        assert (∥ Σ;;; Γ |- array_type a : tSort (sType (Universe.of_level (array_level a))) ∥) as [].
+        assert (∥ Σ;;; Γ |- array_type a : tSort (sType (Universe.of_level (array_universe a))) ∥) as [].
         { sq. eapply checking_typing in X0; eauto.
           erewrite <- abstract_env_ext_wf_universeb_correct in i; tea.
           eapply has_sort_isType; eapply type_Sort; eauto. now move/@wf_universe_reflect: i. }
